NLustre/Stream.v
@@ -108,22 +108,13 @@ if the clocked stream is [absent] at the corresponding instant. *)
     fun n =>
       if beq_nat k (count rs n) then xs n else opaque.
 
-  Remark count_ge_0:
-    forall n r,
-      0 <= count r n.
-  Proof.
-    induction n; simpl; intros.
-    - destruct (r 0); omega.
-    - destruct (r (S n)); auto.
-  Qed.
-
   Corollary count_true_ge_1:
     forall n r,
       r n = true ->
       1 <= count r n.
   Proof.
     induction n; simpl; intros ** E; rewrite E; auto.
-    apply Le.le_n_S, count_ge_0.
+    apply Le.le_n_S; omega.
   Qed.
 
   Lemma count_compat:
